\begin{center}
  \section*{Homework 11 - 7.2, 7.3}
  Due Wed 4/23 \\
  Uzair Hamed Mohammed
\end{center}

\subsection*{7.2 Convergence of Vectors}

2, 3a, 3c, 5a

\begin{enumerate}
  \item[2.] Verify that \(|| \cdot ||_1\) is a norm for
    \(\mathbb{R}^n\) where \(|| x ||_1 = \sum_{i = 1}^{n} |x_i|\).

    \underline{Sol}:\\
    \[
      \begin{array}{l}
        1.\ \text{\textbf{Positivity}:} \\
        \quad ||x||_1 \geq 0,\ \text{and}\ ||x||_1 = 0 \iff x = 0
        \ \text{(since}\ |x_i| \geq 0\ \forall i). \\
        \\
        2.\ \text{\textbf{Scalability}:} \\
        \quad ||\alpha x||_1 = \sum_{i=1}^n |\alpha x_i| =
        |\alpha|\sum_{i=1}^n |x_i| = |\alpha| \cdot ||x||_1. \\
        \\
        3.\ \text{\textbf{Triangle Inequality}:} \\
        \quad ||x + y||_1 = \sum_{i=1}^n |x_i + y_i| \leq
        \sum_{i=1}^n (|x_i| + |y_i|) = ||x||_1 + ||y||_1. \\
        \\
        \therefore\ || \cdot ||_1\ \text{is a norm on}\ \mathbb{R}^n.
      \end{array}
    \]
    \[
      \boxed{|| \cdot ||_1\ \text{is a norm on}\ \mathbb{R}^n}
    \]

  \item[3.] Show that the following sequences are convergent, and
    find their limits.
    \begin{enumerate}
      \item[a.] \(x^{(k)} = (1/k, e^{1 - k}, -2/k^2)^t\)
        \underline{Sol}:\\
        \[
          \begin{aligned}
            &\lim_{k \to \infty} \frac{1}{k} = 0, \quad
            \lim_{k \to \infty} e^{1 - k} = 0, \quad
            \lim_{k \to \infty} \left(-\frac{2}{k^2}\right) = 0. \\
            \Rightarrow \quad &\lim_{k \to \infty} x^{(k)} =
            \begin{pmatrix} 0 \\ 0 \\ 0
            \end{pmatrix}.
          \end{aligned}
        \]
        \[
          \boxed{
            \begin{pmatrix} 0 \\ 0 \\ 0
          \end{pmatrix}}
        \]

      \item[c.] \(x^{(k)} = (ke^{-k^2}, (\cos k)/k, \sqrt{k^2 + k}-k)^t\)

        \underline{Sol}:\\
        \[
          \begin{aligned}
            &\lim_{k \to \infty} ke^{-k^2} = \lim_{k \to \infty}
            \frac{k}{e^{k^2}} = 0 \quad \text{(exponential dominates
            polynomial)}, \\
            &\lim_{k \to \infty} \frac{\cos k}{k} = 0 \quad
            \text{(bounded numerator, divergent denominator)}, \\
            &\lim_{k \to \infty} \left(\sqrt{k^2 + k} - k\right) =
            \lim_{k \to \infty} \frac{k}{\sqrt{k^2 + k} + k} = \frac{1}{2}.
          \end{aligned}
        \]
        \[
          \boxed{
            \begin{pmatrix} 0 \\ 0 \\ \dfrac{1}{2}
          \end{pmatrix}}
        \]
    \end{enumerate}

  \item[5.] The following linear systems \(Ax = b\) have \(x\) as the
    actual solution and \(\tilde{x}\) as an approximate solution.
    Compute \(|| x - \tilde{x}||_\infty\) and \(||A \tilde{x} - b||_\infty\).
    \begin{enumerate}
      \item[a.] \[
          \begin{array}{l}
            \frac{1}{2} x_1 + \frac{1}{3} x_2 = \frac{1}{63}, \\
            \smallbreak \\
            \frac{1}{3} x_1 + \frac{1}{4} x_2 = \frac{1}{168}, \\
            \smallbreak \\
            x = (\frac{1}{7}, - \frac{1}{6})^t, \\
            \smallbreak \\
            \tilde{x} = (0.142, -0.166)^t
          \end{array}
        \]

        \underline{Sol}:\\
        Given \(x = \left(\dfrac{1}{7}, -\dfrac{1}{6}\right)^t\) and
        \(\tilde{x} = (0.142, -0.166)^t\):
        \[
          \begin{aligned}
            ||x - \tilde{x}||_\infty &= \max\left(\left|\dfrac{1}{7}
            - 0.142\right|,\ \left|-\dfrac{1}{6} + 0.166\right|\right) \\
            &= \max\left(\dfrac{3}{3500},\ \dfrac{1}{1500}\right) =
            \dfrac{3}{3500} \approx 0.000857.
          \end{aligned}
        \]
        Compute \(A\tilde{x} - b\):
        \[
          \begin{aligned}
            A\tilde{x} &=
            \begin{pmatrix}
              \dfrac{1}{2}(0.142) + \dfrac{1}{3}(-0.166) \\
              \dfrac{1}{3}(0.142) + \dfrac{1}{4}(-0.166)
            \end{pmatrix} =
            \begin{pmatrix} 0.01567 \\ 0.00583
            \end{pmatrix}, \\
            A\tilde{x} - b &=
            \begin{pmatrix} 0.01567 - \dfrac{1}{63} \\ 0.00583 - \dfrac{1}{168}
            \end{pmatrix} =
            \begin{pmatrix} -0.000206 \\ -0.000119
            \end{pmatrix}.
          \end{aligned}
        \]
        \[
          ||A\tilde{x} - b||_\infty = \max(|-0.000206|,\ |-0.000119|)
          = 0.000206.
        \]
        \[
          \boxed{||x - \tilde{x}||_\infty = 0.000857 \quad \text{and}
          \quad ||A\tilde{x} - b||_\infty = 0.000206}
        \]
    \end{enumerate}
\end{enumerate}

\subsection*{7.3 Eigenvalues and Eigenvectors}

1c, 1e, 3, 5, 7

\begin{enumerate}
  \item[1.] Compute the eigenvalues and associated eigenvectors of
    the following matrices.
    \begin{enumerate}
      \item[c.] \[
          \begin{bmatrix}
            0 & \frac{1}{2} \\
            \frac{1}{2} & 0
          \end{bmatrix}
        \]

        \underline{Sol}:\\
        For \(A =
          \begin{bmatrix} 0 & \frac{1}{2} \\ \frac{1}{2} & 0
        \end{bmatrix}\):
        \[
          \det(A - \lambda I) =
          \begin{vmatrix} -\lambda & \frac{1}{2} \\ \frac{1}{2} & -\lambda
          \end{vmatrix} = \lambda^2 - \frac{1}{4} = 0 \implies
          \lambda = \pm \frac{1}{2}.
        \]
        For \(\lambda = \frac{1}{2}\):
        \[
          (A - \frac{1}{2}I)\mathbf{v} =
          \begin{bmatrix} -\frac{1}{2} & \frac{1}{2} \\ \frac{1}{2} &
            -\frac{1}{2}
          \end{bmatrix}\mathbf{v} = \mathbf{0} \implies v_1 = v_2
          \implies \mathbf{v} = c
          \begin{bmatrix} 1 \\ 1
          \end{bmatrix}.
        \]
        For \(\lambda = -\frac{1}{2}\):
        \[
          (A + \frac{1}{2}I)\mathbf{v} =
          \begin{bmatrix} \frac{1}{2} & \frac{1}{2} \\ \frac{1}{2} &
            \frac{1}{2}
          \end{bmatrix}\mathbf{v} = \mathbf{0} \implies v_1 = -v_2
          \implies \mathbf{v} = c
          \begin{bmatrix} 1 \\ -1
          \end{bmatrix}.
        \]
        \[
          \boxed{\text{Eigenvalues: } \frac{1}{2},\ -\frac{1}{2}
            \quad \text{with eigenvectors }
            \begin{bmatrix} 1 \\ 1
            \end{bmatrix},\
            \begin{bmatrix} 1 \\ -1
          \end{bmatrix}}
        \]

      \item[e.] \[
          \begin{bmatrix}
            2 & 1 & 0 \\
            1 & 2 & 0 \\
            0 & 0 & 3
          \end{bmatrix}
        \]

        \underline{Sol}:\\
        For \(A =
          \begin{bmatrix} 2 & 1 & 0 \\ 1 & 2 & 0 \\ 0 & 0 & 3
        \end{bmatrix}\):
        \[
          \det(A - \lambda I) =
          \begin{vmatrix} 2 - \lambda & 1 & 0 \\ 1 & 2 - \lambda & 0
            \\ 0 & 0 & 3 - \lambda
          \end{vmatrix} = (3 - \lambda)\left[(2 - \lambda)^2 -
          1\right] = (3 - \lambda)(\lambda^2 - 4\lambda + 3).
        \]
        Roots: \(\lambda = 3\) (double), \(\lambda = 1\).

        - For \(\lambda = 3\):
        \[
          (A - 3I)\mathbf{v} =
          \begin{bmatrix} -1 & 1 & 0 \\ 1 & -1 & 0 \\ 0 & 0 & 0
          \end{bmatrix}\mathbf{v} = \mathbf{0} \implies v_1 = v_2,\,
          v_3 \text{ free}. \\
          \text{Eigenvectors: } c_1
          \begin{bmatrix} 1 \\ 1 \\ 0
          \end{bmatrix} + c_2
          \begin{bmatrix} 0 \\ 0 \\ 1
          \end{bmatrix}.
        \]
        - For \(\lambda = 1\):
        \[
          (A - I)\mathbf{v} =
          \begin{bmatrix} 1 & 1 & 0 \\ 1 & 1 & 0 \\ 0 & 0 & 2
          \end{bmatrix}\mathbf{v} = \mathbf{0} \implies v_1 = -v_2,\,
          v_3 = 0. \\
          \text{Eigenvector: } c
          \begin{bmatrix} 1 \\ -1 \\ 0
          \end{bmatrix}.
        \]
        \[
          \boxed{\text{Eigenvalues: } 3,\, 3,\, 1 \quad \text{with
            eigenvectors }
            \begin{bmatrix} 1 \\ 1 \\ 0
            \end{bmatrix},\
            \begin{bmatrix} 0 \\ 0 \\ 1
            \end{bmatrix},\
            \begin{bmatrix} 1 \\ -1 \\ 0
          \end{bmatrix}}
        \]
    \end{enumerate}

  \item[3.] Show that \(A_1 =
      \begin{bmatrix}
        1 & 0 \\
        \frac{1}{4} & \frac{1}{2}
    \end{bmatrix}\) is not convergent, but \(A_2 =
      \begin{bmatrix}
        \frac{1}{2} & 0 \\
        16 & \frac{1}{2}
    \end{bmatrix}\) is convergent.

    \underline{Sol}:\\
    For \(A_1 =
      \begin{bmatrix} 1 & 0 \\ \frac{1}{4} & \frac{1}{2}
    \end{bmatrix}\):
    \[
      \text{Eigenvalues: } \lambda = 1,\ \frac{1}{2} \quad
      (\text{since } \det(A_1 - \lambda I) = (1 -
      \lambda)\left(\frac{1}{2} - \lambda\right) = 0).
    \]
    Spectral radius \(\rho(A_1) = 1 \geq 1\) \(\Rightarrow\) \(A_1\)
    is not convergent.

    For \(A_2 =
      \begin{bmatrix} \frac{1}{2} & 0 \\ 16 & \frac{1}{2}
    \end{bmatrix}\):
    \[
      \text{Eigenvalues: } \lambda = \frac{1}{2},\ \frac{1}{2} \quad
      (\text{repeated; solve } \det(A_2 - \lambda I) =
      \left(\frac{1}{2} - \lambda\right)^2 = 0).
    \]
    Spectral radius \(\rho(A_2) = \frac{1}{2} < 1\) \(\Rightarrow\)
    \(A_2\) is convergent.

  \item[5.] Find the \(|| \cdot ||_2\) norms of the matrices in Exercise 1.
  
  \underline{Sol}:\\
  - Matrix 1(c): \(A = \begin{bmatrix} 0 & \frac{1}{2} \\ \frac{1}{2} & 0 \end{bmatrix}\) \\
    Eigenvalues of \(A\): \(\lambda = \pm \frac{1}{2}\). \\
    Spectral norm \(||A||_2 = \max(|\lambda|) = \frac{1}{2}\). \\

  - Matrix 1(e): \(B = \begin{bmatrix} 2 & 1 & 0 \\ 1 & 2 & 0 \\ 0 & 0 & 3 \end{bmatrix}\) \\
    Eigenvalues of \(B\): \(\lambda = 3, 3, 1\). \\
    Spectral norm \(||B||_2 = \max(|\lambda|) = 3\). \\

  \[
  \boxed{||A||_2 = \dfrac{1}{2} \quad \text{and} \quad ||B||_2 = 3}
  \]

  \item[7.] Find \(2 \times 2\) matrices A and B for which \(\rho (A
    + B) > \rho (A) + \rho (B)\). (This shows that \(\rho (A)\)
    cannot be a matrix norm.)

    \underline{Sol}:\\
    Let \(A = \begin{bmatrix} 0 & 1 \\ 0 & 0 \end{bmatrix}\) and \(B = \begin{bmatrix} 0 & 0 \\ 1 & 0 \end{bmatrix}\).  \\
    - Eigenvalues of \(A\): \(\lambda = 0, 0\) \(\Rightarrow \rho(A) = 0\).  \\
    - Eigenvalues of \(B\): \(\lambda = 0, 0\) \(\Rightarrow \rho(B) = 0\).  \\
    - Sum: \(A + B = \begin{bmatrix} 0 & 1 \\ 1 & 0 \end{bmatrix}\).  \\
      Eigenvalues of \(A + B\): \(\lambda = 1, -1\) \(\Rightarrow \rho(A + B) = 1\).  
    \[
    \rho(A + B) = 1 > \rho(A) + \rho(B) = 0 + 0 = 0.
    \]
    \[
    \boxed{A = \begin{bmatrix} 0 & 1 \\ 0 & 0 \end{bmatrix},\ B = \begin{bmatrix} 0 & 0 \\ 1 & 0 \end{bmatrix}}
    \]

\end{enumerate}
